fix floyd/local2ptree_(eval, typecheck).v

floyd/local2ptree_typecheck.v
@@ -6,28 +6,32 @@ Require Import VST.floyd.local2ptree_denote.
 Require Import VST.floyd.local2ptree_eval.
 
 Import LiftNotation.
-Import compcert.lib.Maps.
-Local Open Scope logic.
+Import -(notations) compcert.lib.Maps.
+
+
+
+Section MSUBST_DENOTE_TC_ASSERT.
+
+Context `{!heapGS Σ}.
+Context {cs: compspecs} (Delta: tycontext) (T1: PTree.t val) (T2: PTree.t (type * val)) (GV: option globals).
 
 Definition msubst_simpl_tc_assert (T1: PTree.t val): tc_assert -> tc_assert :=
   fix msubst_simpl_tc_assert (tc: tc_assert): tc_assert :=
   match tc with
   | tc_andp' tc1 tc2 => tc_andp (msubst_simpl_tc_assert tc1) (msubst_simpl_tc_assert tc2)
   | tc_orp' tc1 tc2 => tc_orp (msubst_simpl_tc_assert tc1) (msubst_simpl_tc_assert tc2)
-  | tc_initialized i _ => match T1 ! i with Some _ => tc_TT | None => tc_FF miscellaneous_typecheck_error end
+  | tc_initialized i _ => match T1 !! i with Some _ => tc_TT | None => tc_FF miscellaneous_typecheck_error end
   | _ => tc
   end.
 
-Section MSUBST_DENOTE_TC_ASSERT.
 
-Context {cs: compspecs} (Delta: tycontext) (T1: PTree.t val) (T2: PTree.t (type * val)) (GV: option globals).
 
 Fixpoint msubst_denote_tc_assert (tc: tc_assert): mpred :=
   match tc with
-  | tc_FF msg => !! (typecheck_error msg)
-  | tc_TT => TT
-  | tc_andp' b c => (msubst_denote_tc_assert b) && (msubst_denote_tc_assert c)
-  | tc_orp' b c => (msubst_denote_tc_assert b) || (msubst_denote_tc_assert c)
+  | tc_FF msg => ⌜typecheck_error msg⌝
+  | tc_TT => True
+  | tc_andp' b c => (msubst_denote_tc_assert b) ∧ (msubst_denote_tc_assert c)
+  | tc_orp' b c => (msubst_denote_tc_assert b) ∨ (msubst_denote_tc_assert c)
   | tc_nonzero' e => denote_tc_nonzero (force_val (msubst_eval_expr Delta T1 T2 GV e))
   | tc_isptr e => denote_tc_isptr (force_val (msubst_eval_expr Delta T1 T2 GV e))
   | tc_isint e => denote_tc_isint (force_val (msubst_eval_expr Delta T1 T2 GV e))
@@ -40,7 +44,7 @@ Fixpoint msubst_denote_tc_assert (tc: tc_assert): mpred :=
   | tc_Zge e z => denote_tc_Zle z (force_val (msubst_eval_expr Delta T1 T2 GV e))
   | tc_samebase e1 e2 => denote_tc_samebase (force_val (msubst_eval_expr Delta T1 T2 GV e1)) (force_val (msubst_eval_expr Delta T1 T2 GV e2))
   | tc_nodivover' v1 v2 => denote_tc_nodivover (force_val (msubst_eval_expr Delta T1 T2 GV v1)) (force_val (msubst_eval_expr Delta T1 T2 GV v2))
-  | tc_initialized id ty => FF
+  | tc_initialized id ty => False
   | tc_iszero' e => denote_tc_iszero (force_val (msubst_eval_expr Delta T1 T2 GV e))
   | tc_nosignedover op e1 e2 => 
      match typeof e1, typeof e2 with
@@ -76,295 +80,204 @@ Definition msubst_tc_expropt (e: option expr) (t: type) :=
      end)).
 
 (* Soundness proof *)
-
-Lemma msubst_denote_tc_assert_sound: forall P R tc,
-  local (tc_environ Delta) && PROPx P (LOCALx (LocalD T1 T2 GV) (SEPx R)) && `(msubst_denote_tc_assert tc) |--
-    denote_tc_assert tc.
+Lemma denote_tc_assert_andp': forall P Q,
+  denote_tc_assert (tc_andp' P Q) ⊣⊢ denote_tc_assert P ∧ denote_tc_assert Q.
 Proof.
   intros.
+  simpl. unfold_lift. raise_rho. done.
+Qed.
+
+Lemma lift_or: forall P Q,
+  assert_of(Σ:=Σ) `(P ∨ Q) ⊣⊢ (assert_of `(P) ∨ (assert_of `(Q))).
+Proof.
+  intros. unfold_lift. raise_rho. done.
+Qed.
+
+Lemma derives_trans: forall {prop:bi} (P Q R:prop),
+  (P -∗ Q) -> (Q -∗ R) -> (P -∗ R).
+Proof. intros. rewrite H H0 //. Qed.
+
+Lemma msubst_denote_tc_assert_sound: forall P R tc,
+  local (tc_environ Delta) ∧ PROPx P (LOCALx (LocalD T1 T2 GV) (SEPx R)) ∧ (assert_of `(msubst_denote_tc_assert tc)) ⊢
+    denote_tc_assert tc.
+Proof.
+  Ltac and_elim_rightmost := 
+    rewrite bi.and_elim_l; apply bi.impl_intro_r; rewrite bi.and_elim_r;
+    simpl denote_tc_nonzero; unfold local, lift1; unfold_lift; raise_rho;
+    normalize.
+  intros.
   induction tc.
-  + apply andp_left2; apply derives_refl.
-  + apply andp_left2; apply derives_refl.
-  + change (denote_tc_assert (tc_andp' tc1 tc2)) with (denote_tc_assert tc1 && denote_tc_assert tc2).
-    change (`(msubst_denote_tc_assert (tc_andp' tc1 tc2)))
-      with (`(msubst_denote_tc_assert tc1) && `(msubst_denote_tc_assert tc2)).
-    apply andp_right.
-    - eapply derives_trans; [| apply IHtc1].
+  + rewrite !bi.and_elim_r. done.
+  + rewrite !bi.and_elim_r. done.
+  + rewrite denote_tc_assert_andp'.
+    apply bi.and_intro.
+    - rewrite -IHtc1 /=. rewrite bi.and_mono //. rewrite bi.and_mono //. 
+      unfold_lift. raise_rho. simpl.
       solve_andp.
-    - eapply derives_trans; [| apply IHtc2].
+    - rewrite -IHtc2 /=. rewrite bi.and_mono //. rewrite bi.and_mono //. 
+      unfold_lift. raise_rho. simpl.
       solve_andp.
-  + change (denote_tc_assert (tc_orp' tc1 tc2)) with (denote_tc_assert tc1 || denote_tc_assert tc2).
-    change (`(msubst_denote_tc_assert (tc_orp' tc1 tc2)))
-      with (`(msubst_denote_tc_assert tc1) || `(msubst_denote_tc_assert tc2)).
-    rewrite (andp_comm (_ && _)).
-    apply imp_andp_adjoint.
-    apply orp_left; apply imp_andp_adjoint; rewrite <- (andp_comm (_ && _)).
-    - eapply derives_trans; [exact IHtc1 | apply orp_right1; auto].
-    - eapply derives_trans; [exact IHtc2 | apply orp_right2; auto].
+  + simpl (` (msubst_denote_tc_assert _)).
+    rewrite lift_or.
+    rewrite bi.and_assoc.
+    rewrite bi.and_or_l.
+    apply bi.or_elim; rewrite -bi.and_assoc.
+    - rewrite IHtc1. split => rho. simpl. unfold_lift. apply bi.or_intro_l.
+    - rewrite IHtc2. split => rho. simpl. unfold_lift. apply bi.or_intro_r.
   + simpl msubst_denote_tc_assert; simpl denote_tc_assert.
-    apply imp_andp_adjoint.
+    rewrite bi.and_assoc. apply bi.impl_elim_l'.
     destruct (msubst_eval_expr Delta T1 T2 GV e) eqn:?H.
     - eapply derives_trans; [eapply msubst_eval_expr_eq; eauto |].
-      apply imp_andp_adjoint.
+      apply bi.impl_intro_r.
       unfold local, lift1; unfold_lift.
-      intros rho.
-      simpl.
       normalize.
-    - apply andp_left1, imp_andp_adjoint, andp_left2.
-      simpl denote_tc_nonzero.
-      unfold local, lift1; unfold_lift.
-      intros rho.
-      simpl.
-      normalize.
+    - and_elim_rightmost.
   + simpl msubst_denote_tc_assert; simpl denote_tc_assert.
-    apply imp_andp_adjoint.
+    rewrite bi.and_assoc. apply bi.impl_elim_l'.
     destruct (msubst_eval_expr Delta T1 T2 GV e) eqn:?H.
     - eapply derives_trans; [eapply msubst_eval_expr_eq; eauto |].
-      apply imp_andp_adjoint.
+      apply bi.impl_intro_l.
       unfold local, lift1; unfold_lift.
-      intros rho.
-      simpl.
+      raise_rho.
       normalize.
-    - apply andp_left1, imp_andp_adjoint, andp_left2.
-      simpl denote_tc_iszero.
-      unfold local, lift1; unfold_lift.
-      intros rho.
-      simpl.
-      normalize.
+    - and_elim_rightmost.
   + simpl msubst_denote_tc_assert; simpl denote_tc_assert.
-    apply imp_andp_adjoint.
+    rewrite bi.and_assoc. apply bi.impl_elim_l'.
     destruct (msubst_eval_expr Delta T1 T2 GV e) eqn:?H.
     - eapply derives_trans; [eapply msubst_eval_expr_eq; eauto |].
-      apply imp_andp_adjoint.
+      apply bi.impl_intro_l.
       unfold local, lift1; unfold_lift.
-      intros rho.
-      simpl.
+      raise_rho.
       normalize.
-    - apply andp_left1, imp_andp_adjoint, andp_left2.
-      unfold denote_tc_isptr.
-      unfold local, lift1; unfold_lift.
-      intros rho.
-      simpl.
-      normalize.
+    - and_elim_rightmost.
   + simpl msubst_denote_tc_assert; simpl denote_tc_assert.
-    apply imp_andp_adjoint.
+    rewrite bi.and_assoc. apply bi.impl_elim_l'.
     destruct (msubst_eval_expr Delta T1 T2 GV e) eqn:?H.
     - eapply derives_trans; [eapply msubst_eval_expr_eq; eauto |].
-      apply imp_andp_adjoint.
+      apply bi.impl_intro_l.
       unfold local, lift1; unfold_lift.
-      intros rho.
-      simpl.
+      raise_rho.
       normalize.
-    - apply andp_left1, imp_andp_adjoint, andp_left2.
-      unfold denote_tc_isint.
-      unfold local, lift1; unfold_lift.
-      intros rho.
-      simpl.
-      normalize.
+    - and_elim_rightmost.
   + simpl msubst_denote_tc_assert; simpl denote_tc_assert.
-    apply imp_andp_adjoint.
+    rewrite bi.and_assoc. apply bi.impl_elim_l'.
     destruct (msubst_eval_expr Delta T1 T2 GV e) eqn:?H.
     - eapply derives_trans; [eapply msubst_eval_expr_eq; eauto |].
-      apply imp_andp_adjoint.
+      apply bi.impl_intro_l.
       unfold local, lift1; unfold_lift.
-      intros rho.
-      simpl.
+      raise_rho.
       normalize.
-    - apply andp_left1, imp_andp_adjoint, andp_left2.
-      unfold denote_tc_islong.
-      unfold local, lift1; unfold_lift.
-      intros rho.
-      simpl.
-      normalize.
+    - and_elim_rightmost.
   + simpl msubst_denote_tc_assert; simpl denote_tc_assert.
-    apply imp_andp_adjoint.
+    rewrite bi.and_assoc. apply bi.impl_elim_l'.
     destruct (msubst_eval_expr Delta T1 T2 GV e) eqn:?H, (msubst_eval_expr Delta T1 T2 GV e0) eqn:?H.
-    - eapply derives_trans; [apply andp_right; eapply msubst_eval_expr_eq; [exact H | exact H0] |].
-      rewrite <- imp_andp_adjoint.
+    - eapply derives_trans; [apply bi.and_intro; eapply msubst_eval_expr_eq; [exact H | exact H0] |].
+      apply bi.impl_intro_l.
       unfold local, lift1; unfold_lift.
-      intros rho.
-      simpl.
+      raise_rho.
       normalize.
-    - apply andp_left1, imp_andp_adjoint, andp_left2.
-      unfold denote_tc_test_eq.
-      unfold local, lift1; unfold_lift.
-      intros rho.
+    - and_elim_rightmost.
       destruct v; simpl; normalize.
-    - apply andp_left1, imp_andp_adjoint, andp_left2.
-      unfold denote_tc_test_eq.
-      unfold local, lift1; unfold_lift.
-      intros rho.
-      destruct v; simpl; normalize.
-    - apply andp_left1, imp_andp_adjoint, andp_left2.
-      unfold denote_tc_test_eq.
-      unfold local, lift1; unfold_lift.
-      intros rho.
-      simpl; normalize.
+    - and_elim_rightmost.
+    - and_elim_rightmost.
   + simpl msubst_denote_tc_assert; simpl denote_tc_assert.
-    apply imp_andp_adjoint.
+    rewrite bi.and_assoc. apply bi.impl_elim_l'.
     destruct (msubst_eval_expr Delta T1 T2 GV e) eqn:?H, (msubst_eval_expr Delta T1 T2 GV e0) eqn:?H.
-    - eapply derives_trans; [apply andp_right; eapply msubst_eval_expr_eq; [exact H | exact H0] |].
-      rewrite <- imp_andp_adjoint.
+    - eapply derives_trans; [apply bi.and_intro; eapply msubst_eval_expr_eq; [exact H | exact H0] |].
+      apply bi.impl_intro_l.
       unfold local, lift1; unfold_lift.
-      intros rho.
-      simpl.
+      raise_rho.
       normalize.
-    - apply andp_left1, imp_andp_adjoint, andp_left2.
+    - and_elim_rightmost.
       unfold denote_tc_test_order.
-      unfold local, lift1; unfold_lift.
-      intros rho.
       destruct v; simpl; normalize.
-    - apply andp_left1, imp_andp_adjoint, andp_left2.
-      unfold denote_tc_test_order.
-      unfold local, lift1; unfold_lift.
-      intros rho.
-      destruct v; simpl; normalize.
-    - apply andp_left1, imp_andp_adjoint, andp_left2.
-      unfold denote_tc_test_order.
-      unfold local, lift1; unfold_lift.
-      intros rho.
-      simpl; normalize.
+    - and_elim_rightmost.
+    - and_elim_rightmost.
   + simpl msubst_denote_tc_assert; simpl denote_tc_assert.
-    apply imp_andp_adjoint.
+    rewrite bi.and_assoc. apply bi.impl_elim_l'.
     destruct (msubst_eval_expr Delta T1 T2 GV e) eqn:?H.
     - eapply derives_trans; [eapply msubst_eval_expr_eq; eauto |].
-      apply imp_andp_adjoint.
+      apply bi.impl_intro_l.
       unfold local, lift1; unfold_lift.
-      intros rho.
-      simpl.
+      raise_rho.
       normalize.
-    - apply andp_left1, imp_andp_adjoint, andp_left2.
-      simpl denote_tc_igt.
-      unfold local, lift1; unfold_lift.
-      intros rho.
-      simpl.
-      normalize.
+    - and_elim_rightmost.
   + simpl msubst_denote_tc_assert; simpl denote_tc_assert.
-    apply imp_andp_adjoint.
+    rewrite bi.and_assoc. apply bi.impl_elim_l'.
     destruct (msubst_eval_expr Delta T1 T2 GV e) eqn:?H.
     - eapply derives_trans; [eapply msubst_eval_expr_eq; eauto |].
-      apply imp_andp_adjoint.
+      apply bi.impl_intro_l.
       unfold local, lift1; unfold_lift.
-      intros rho.
-      simpl.
+      raise_rho.
       normalize.
-    - apply andp_left1, imp_andp_adjoint, andp_left2.
-      simpl denote_tc_Zge.
-      unfold local, lift1; unfold_lift.
-      intros rho.
-      simpl.
-      normalize.
+    - and_elim_rightmost.
   + simpl msubst_denote_tc_assert; simpl denote_tc_assert.
-    apply imp_andp_adjoint.
+    rewrite bi.and_assoc. apply bi.impl_elim_l'.
     destruct (msubst_eval_expr Delta T1 T2 GV e) eqn:?H.
     - eapply derives_trans; [eapply msubst_eval_expr_eq; eauto |].
-      apply imp_andp_adjoint.
+      apply bi.impl_intro_l.
       unfold local, lift1; unfold_lift.
-      intros rho.
-      simpl.
+      raise_rho.
       normalize.
-    - apply andp_left1, imp_andp_adjoint, andp_left2.
-      simpl denote_tc_Zle.
-      unfold local, lift1; unfold_lift.
-      intros rho.
-      simpl.
-      normalize.
+    - and_elim_rightmost.
   + simpl msubst_denote_tc_assert; simpl denote_tc_assert.
-    apply imp_andp_adjoint.
+    rewrite bi.and_assoc. apply bi.impl_elim_l'.
     destruct (msubst_eval_expr Delta T1 T2 GV e) eqn:?H.
     - eapply derives_trans; [eapply msubst_eval_expr_eq; eauto |].
-      apply imp_andp_adjoint.
+      apply bi.impl_intro_l.
       unfold local, lift1; unfold_lift.
-      intros rho.
-      simpl.
+      raise_rho.
       normalize.
-    - apply andp_left1, imp_andp_adjoint, andp_left2.
-      simpl denote_tc_Zle.
-      unfold local, lift1; unfold_lift.
-      intros rho.
-      simpl.
-      normalize.
+    - and_elim_rightmost.
   + simpl msubst_denote_tc_assert; simpl denote_tc_assert.
-    apply imp_andp_adjoint.
+    rewrite bi.and_assoc. apply bi.impl_elim_l'.
     destruct (msubst_eval_expr Delta T1 T2 GV e) eqn:?H, (msubst_eval_expr Delta T1 T2 GV e0) eqn:?H.
-    - eapply derives_trans; [apply andp_right; eapply msubst_eval_expr_eq; [exact H | exact H0] |].
-      rewrite <- imp_andp_adjoint.
+    - eapply derives_trans; [apply bi.and_intro; eapply msubst_eval_expr_eq; [exact H | exact H0] |].
+      apply bi.impl_intro_l.
       unfold local, lift1; unfold_lift.
-      intros rho.
-      simpl.
+      raise_rho.
       normalize.
-    - apply andp_left1, imp_andp_adjoint, andp_left2.
+    - and_elim_rightmost.
       unfold denote_tc_samebase.
-      unfold local, lift1; unfold_lift.
-      intros rho.
       destruct v; simpl; normalize.
-    - apply andp_left1, imp_andp_adjoint, andp_left2.
-      unfold denote_tc_samebase.
-      unfold local, lift1; unfold_lift.
-      intros rho.
-      destruct v; simpl; normalize.
-    - apply andp_left1, imp_andp_adjoint, andp_left2.
-      unfold denote_tc_samebase.
-      unfold local, lift1; unfold_lift.
-      intros rho.
-      simpl; normalize.
+    - and_elim_rightmost.
+    - and_elim_rightmost.
   + simpl msubst_denote_tc_assert; simpl denote_tc_assert.
-    apply imp_andp_adjoint.
+    rewrite bi.and_assoc. apply bi.impl_elim_l'.
     destruct (msubst_eval_expr Delta T1 T2 GV e) eqn:?H, (msubst_eval_expr Delta T1 T2 GV e0) eqn:?H.
-    - eapply derives_trans; [apply andp_right; eapply msubst_eval_expr_eq; [exact H | exact H0] |].
-      rewrite <- imp_andp_adjoint.
+    - eapply derives_trans; [apply bi.and_intro; eapply msubst_eval_expr_eq; [exact H | exact H0] |].
+      apply bi.impl_intro_l.
       unfold local, lift1; unfold_lift.
-      intros rho.
-      simpl.
+      raise_rho.
       normalize.
-    - apply andp_left1, imp_andp_adjoint, andp_left2.
+    - and_elim_rightmost.
       unfold denote_tc_nodivover.
-      unfold local, lift1; unfold_lift.
-      intros rho.
       destruct v; simpl; normalize.
-    - apply andp_left1, imp_andp_adjoint, andp_left2.
-      unfold denote_tc_nodivover.
-      unfold local, lift1; unfold_lift.
-      intros rho.
-      destruct v; simpl; normalize.
-    - apply andp_left1, imp_andp_adjoint, andp_left2.
-      unfold denote_tc_nodivover.
-      unfold local, lift1; unfold_lift.
-      intros rho.
-      simpl; normalize.
+    - and_elim_rightmost.
+    - and_elim_rightmost.
   + simpl msubst_denote_tc_assert; simpl denote_tc_assert.
     unfold local, lift1; unfold_lift.
-    intros rho.
-    simpl; normalize.
+    raise_rho.
+    normalize.
   + simpl msubst_denote_tc_assert; simpl denote_tc_assert.
-    apply imp_andp_adjoint.
+    rewrite bi.and_assoc. apply bi.impl_elim_l'.
     destruct (msubst_eval_expr Delta T1 T2 GV e) eqn:?H, (msubst_eval_expr Delta T1 T2 GV e0) eqn:?H.
-    - eapply derives_trans; [apply andp_right; eapply msubst_eval_expr_eq; [exact H | exact H0] |].
-      rewrite <- imp_andp_adjoint.
+    - eapply derives_trans; [apply bi.and_intro; eapply msubst_eval_expr_eq; [exact H | exact H0] |].
+      apply bi.impl_intro_l.
       unfold local, lift1; unfold_lift.
-      intros rho.
-      simpl.
+      raise_rho.
       normalize.
      destruct (typeof e) as [ | _ [ | ] _ | | | | | | | ],
        (typeof e0) as [ | _ [ | ] _ | | | | | | | ]; simpl; normalize.
-    - apply andp_left1, imp_andp_adjoint, andp_left2.
-      unfold denote_tc_samebase.
-      unfold local, lift1; unfold_lift.
-      intros rho.
+    - and_elim_rightmost.
      destruct (typeof e) as [ | _ [ | ] _ | | | | | | | ],
        (typeof e0) as [ | _ [ | ] _ | | | | | | | ],
          v; simpl; normalize.
-    - apply andp_left1, imp_andp_adjoint, andp_left2.
-      unfold denote_tc_samebase.
-      unfold local, lift1; unfold_lift.
-      intros rho.
+    - and_elim_rightmost.
      destruct (typeof e) as [ | _ [ | ] _ | | | | | | | ],
        (typeof e0) as [ | _ [ | ] _ | | | | | | | ],
          v; simpl; normalize.
-    - apply andp_left1, imp_andp_adjoint, andp_left2.
-      unfold denote_tc_samebase.
-      unfold local, lift1; unfold_lift.
-      intros rho.
+    - and_elim_rightmost.
      destruct (typeof e) as [ | _ [ | ] _ | | | | | | | ],
        (typeof e0) as [ | _ [ | ] _ | | | | | | | ];
       simpl; normalize.
@@ -372,70 +285,73 @@ Qed.
 
 End MSUBST_DENOTE_TC_ASSERT.
 
+Section MSUBST_TC.
+Context `{!heapGS Σ}.
 Definition legal_tc_init (Delta: tycontext): tc_assert -> Prop :=
   fix legal_tc_init (tc: tc_assert): Prop :=
   match tc with
   | tc_andp' tc1 tc2 => legal_tc_init tc1 /\ legal_tc_init tc2
   | tc_orp' tc1 tc2 => legal_tc_init tc1 /\ legal_tc_init tc2
-  | tc_initialized i t => (temp_types Delta) ! i = Some t
-  | _ => True
+  | tc_initialized i t => (temp_types Delta) !! i = Some t
+  | _ => True:Prop
   end.
 
 Lemma temp_tc_initialized: forall Delta i t v,
-  (temp_types Delta) ! i = Some t ->
-  local (tc_environ Delta) && local (locald_denote (temp i v))
-    |-- denote_tc_initialized i t.
+  (temp_types Delta) !! i = Some t ->
+  local (tc_environ Delta) ∧ local (locald_denote (temp i v))
+    ⊢ assert_of (denote_tc_initialized i t).
 Proof.
   intros.
-  intros rho.
   unfold local, lift1; simpl; unfold_lift; simpl.
-  normalize.
-  unfold denote_tc_initialized.
-  apply prop_right.
+  raise_rho.
+  iIntros "[%H0 %H1]".
+  iPureIntro.
   destruct H0 as [? _].
   specialize (H0 _ _ H).
-  destruct H0 as [v [? ?]].
+  destruct H0 as [v' [? ?]].
   unfold eval_id, force_val in H1.
-  rewrite H0 in *.
+  rewrite -> H0 in *.
+  destruct H1 as [Hv H1]; subst.
   specialize (H2 H1).
   eauto.
 Qed.
-
+Print derives_refl.
 Lemma msubst_simpl_tc_assert_sound: forall {cs: compspecs} Delta P T1 T2 Q R tc,
   legal_tc_init Delta tc ->
-  local (tc_environ Delta) && PROPx P (LOCALx (LocalD T1 T2 Q) (SEPx R)) &&
-    denote_tc_assert (msubst_simpl_tc_assert T1 tc) |--
+  local (tc_environ Delta) ∧ PROPx P (LOCALx (LocalD T1 T2 Q) (SEPx R)) ∧
+    denote_tc_assert (msubst_simpl_tc_assert T1 tc) ⊢
   denote_tc_assert tc.
 Proof.
   intros.
-  induction tc; try solve [apply andp_left2, derives_refl].
+  induction tc; try solve [rewrite bi.and_assoc; apply bi.and_elim_r; apply derives_refl].
   + inversion H.
     simpl msubst_simpl_tc_assert.
+    rewrite denote_tc_assert_andp'.
     rewrite denote_tc_assert_andp.
-    change (denote_tc_assert (tc_andp' tc1 tc2)) with
-      (denote_tc_assert tc1 && denote_tc_assert tc2).
-    apply andp_right.
-    - eapply derives_trans; [| apply IHtc1, H0].
+    apply bi.and_intro.
+    - iIntros "H". iApply (IHtc1 with "[H]"). iStopProof.
+      raise_rho.
       solve_andp.
-    - eapply derives_trans; [| apply IHtc2, H1].
+    - iIntros "H". iApply (IHtc2 with "[H]"). iStopProof.
+      raise_rho.
       solve_andp.
   + inversion H.
     simpl msubst_simpl_tc_assert.
     rewrite denote_tc_assert_orp.
-    change (denote_tc_assert (tc_orp' tc1 tc2)) with
-      (denote_tc_assert tc1 || denote_tc_assert tc2).
-    rewrite (andp_comm (_ && _)).
-    apply imp_andp_adjoint.
-    apply orp_left; apply imp_andp_adjoint; rewrite <- (andp_comm (_ && _)).
-    - eapply derives_trans; [apply IHtc1, H0 | apply orp_right1; auto].
-    - eapply derives_trans; [apply IHtc2, H1 | apply orp_right2; auto].
+    rewrite bi.and_assoc.
+    rewrite bi.and_or_l.
+    apply bi.or_elim; rewrite -bi.and_assoc.
+    - rewrite (IHtc1 H0). raise_rho. simpl. unfold_lift. apply bi.or_intro_l.
+    - rewrite (IHtc2 H1). raise_rho. simpl. unfold_lift. apply bi.or_intro_r.
   + inv H.
     simpl denote_tc_assert.
-    destruct (T1 ! e) eqn:?H; [apply andp_left1 | simpl; intros; apply andp_left2, FF_left].
-    apply (LocalD_sound_temp _ _ _ T2 Q) in H.
-    rewrite (add_andp _ _ (in_local _ _ _ _ _ H)).
-    eapply derives_trans; [| apply (temp_tc_initialized Delta _ _ v); eauto].
-    solve_andp.
+    destruct (T1 !! e) eqn:?H.
+    - rewrite bi.and_assoc; rewrite bi.and_elim_l.
+      apply (LocalD_sound_temp _ _ _ T2 Q) in H.
+      rewrite (add_andp _ _ (in_local _ _ _ _ _ H)).
+      eapply derives_trans; [| apply (temp_tc_initialized Delta _ _ v); eauto].
+      solve_andp.
+    - simpl; intros; rewrite bi.and_assoc; rewrite bi.and_elim_r. raise_rho. apply bi.False_elim. 
 Qed.
 
 Lemma legal_tc_init_tc_bool: forall Delta b err,
@@ -539,7 +455,7 @@ Qed.
 
 Ltac solve_legal_tc_init :=
   repeat progress
-   (simpl; auto;
+   (simpl; auto; unfold typecheck_lvalue; unfold typecheck_expr;
       match goal with
       | |- context [match ?A with _ => _ end] => destruct A eqn:?H
       | |- legal_tc_init _ (tc_bool _ _) => apply legal_tc_init_tc_bool
@@ -618,72 +534,89 @@ Proof.
 Qed.
 
 Lemma msubst_tc_lvalue_sound: forall {cs: compspecs} Delta P T1 T2 GV R e,
-  local (tc_environ Delta) && PROPx P (LOCALx (LocalD T1 T2 GV) (SEPx R)) && ` (msubst_tc_lvalue Delta T1 T2 GV e) |--
+  local (tc_environ Delta) ∧ PROPx P (LOCALx (LocalD T1 T2 GV) (SEPx R)) ∧ (assert_of `(msubst_tc_lvalue Delta T1 T2 GV e)) ⊢
     tc_lvalue Delta e.
 Proof.
   intros.
   eapply derives_trans; [| apply msubst_simpl_tc_assert_sound, typecheck_lvalue_legal_tc_init].
-  apply andp_right; [apply andp_left1; apply derives_refl | ].
+  rewrite [in X in X -∗ _]bi.and_assoc.
+  rewrite [in X in _ -∗ X]bi.and_assoc.
+  apply bi.and_intro; [rewrite bi.and_elim_l; apply derives_refl | ].
+  rewrite -bi.and_assoc.
   apply msubst_denote_tc_assert_sound.
 Qed.
 
 Lemma msubst_tc_expr_sound: forall {cs: compspecs} Delta P T1 T2 GV R e,
-  local (tc_environ Delta) && PROPx P (LOCALx (LocalD T1 T2 GV) (SEPx R)) && ` (msubst_tc_expr Delta T1 T2 GV e) |--
+  local (tc_environ Delta) ∧ PROPx P (LOCALx (LocalD T1 T2 GV) (SEPx R)) ∧ (assert_of `(msubst_tc_expr Delta T1 T2 GV e)) ⊢
     tc_expr Delta e.
 Proof.
   intros.
   eapply derives_trans; [| apply msubst_simpl_tc_assert_sound, typecheck_expr_legal_tc_init].
-  apply andp_right; [apply andp_left1; apply derives_refl | ].
+  rewrite [in X in X -∗ _]bi.and_assoc.
+  rewrite [in X in _ -∗ X]bi.and_assoc.
+  apply bi.and_intro; [rewrite bi.and_elim_l; apply derives_refl | ].
+  rewrite -bi.and_assoc.
   apply msubst_denote_tc_assert_sound.
 Qed.
 
 Lemma msubst_tc_LR_sound: forall {cs: compspecs} Delta P T1 T2 GV R e lr,
-  local (tc_environ Delta) && PROPx P (LOCALx (LocalD T1 T2 GV) (SEPx R)) && ` (msubst_tc_LR Delta T1 T2 GV e lr) |--
+  local (tc_environ Delta) ∧ PROPx P (LOCALx (LocalD T1 T2 GV) (SEPx R)) ∧ (assert_of `(msubst_tc_LR Delta T1 T2 GV e lr)) ⊢
     tc_LR Delta e lr.
 Proof.
   intros.
   eapply derives_trans; [| apply msubst_simpl_tc_assert_sound, typecheck_LR_legal_tc_init].
-  apply andp_right; [apply andp_left1; apply derives_refl | ].
+  rewrite [in X in X -∗ _]bi.and_assoc.
+  rewrite [in X in _ -∗ X]bi.and_assoc.
+  apply bi.and_intro; [rewrite bi.and_elim_l; apply derives_refl | ].
+  rewrite -bi.and_assoc.
   apply msubst_denote_tc_assert_sound.
 Qed.
 
 Lemma msubst_tc_efield_sound: forall {cs: compspecs} Delta P T1 T2 GV R efs,
-  local (tc_environ Delta) && PROPx P (LOCALx (LocalD T1 T2 GV) (SEPx R)) && ` (msubst_tc_efield Delta T1 T2 GV efs) |--
-    tc_efield Delta efs.
+  local (tc_environ Delta) ∧ PROPx P (LOCALx (LocalD T1 T2 GV) (SEPx R)) ∧ (assert_of `(msubst_tc_efield Delta T1 T2 GV efs)) ⊢
+    (assert_of (tc_efield Delta efs)).
 Proof.
   intros.
   eapply derives_trans; [| apply msubst_simpl_tc_assert_sound, typecheck_efield_legal_tc_init].
-  apply andp_right; [apply andp_left1; apply derives_refl | ].
+  rewrite [in X in X -∗ _]bi.and_assoc.
+  rewrite [in X in _ -∗ X]bi.and_assoc.
+  apply bi.and_intro; [rewrite bi.and_elim_l; apply derives_refl | ].
+  rewrite -bi.and_assoc.
   apply msubst_denote_tc_assert_sound.
 Qed.
 
 Lemma msubst_tc_exprlist_sound: forall {cs: compspecs} Delta P T1 T2 GV R ts es,
-  local (tc_environ Delta) && PROPx P (LOCALx (LocalD T1 T2 GV) (SEPx R)) && ` (msubst_tc_exprlist Delta T1 T2 GV ts es) |--
+  local (tc_environ Delta) ∧ PROPx P (LOCALx (LocalD T1 T2 GV) (SEPx R)) ∧ (assert_of `(msubst_tc_exprlist Delta T1 T2 GV ts es)) ⊢
     tc_exprlist Delta ts es.
 Proof.
   intros.
   eapply derives_trans; [| apply msubst_simpl_tc_assert_sound, typecheck_exprlist_legal_tc_init].
-  apply andp_right; [apply andp_left1; apply derives_refl | ].
+  rewrite [in X in X -∗ _]bi.and_assoc.
+  rewrite [in X in _ -∗ X]bi.and_assoc.
+  apply bi.and_intro; [rewrite bi.and_elim_l; apply derives_refl | ].
+  rewrite -bi.and_assoc.
   apply msubst_denote_tc_assert_sound.
 Qed.
 
 Lemma msubst_tc_expropt_sound: forall {cs: compspecs} Delta P T1 T2 GV R t e,
-  local (tc_environ Delta) && PROPx P (LOCALx (LocalD T1 T2 GV) (SEPx R)) && ` (msubst_tc_expropt Delta T1 T2 GV e t) |--
+  local (tc_environ Delta) ∧ PROPx P (LOCALx (LocalD T1 T2 GV) (SEPx R)) ∧ (assert_of `(msubst_tc_expropt Delta T1 T2 GV e t)) ⊢
     tc_expropt Delta e t.
 Proof.
   intros.
   unfold msubst_tc_expropt, msubst_tc_expr, tc_expropt.
   destruct e.
   + eapply derives_trans; [| apply msubst_simpl_tc_assert_sound, typecheck_expr_legal_tc_init].
-    apply andp_right; [apply andp_left1; apply derives_refl | ].
+    rewrite [in X in X -∗ _]bi.and_assoc.
+    rewrite [in X in _ -∗ X]bi.and_assoc.
+    apply bi.and_intro; [rewrite bi.and_elim_l; apply derives_refl | ].
+    rewrite -bi.and_assoc.
     apply msubst_denote_tc_assert_sound.
   + destruct (eqb_type t Tvoid) eqn:?H.
     - rewrite eqb_type_spec in H.
       subst.
-      simpl; intro.
-      unfold_lift.
-      normalize.
-    - simpl; intro.
+      iIntros; done.
+    - raise_rho.
       unfold_lift.
       normalize.
 Qed.
+End MSUBST_TC.
